add proofs for tactic theorems

src/Iris/Proofmode/Environments.lean
@@ -26,30 +26,37 @@ def length : Env α → Nat
   | .nil       => 0
   | .cons _ as => as.length + 1
 
+theorem length_cons_list_cons {a : α} {as : List α} {b : β} {bs : Env β} :
+  (a :: as).length = (Env.cons b bs).length →
+  as.length = bs.length
+:= by
+  intro h
+  simp only [length, List.length] at h
+  rw [Nat.add_right_cancel h]
+
 @[reducible]
-def eraseIdx : (e : Env α) → Fin (e.length) → Env α
+def eraseIdx : (Γ : Env α) → Fin (Γ.length) → Env α
   | .cons _ as, ⟨0    , _⟩ => as
   | .cons a as, ⟨i + 1, h⟩ => .cons a <| as.eraseIdx ⟨i, Nat.le_of_succ_le_succ h⟩
 
 @[reducible]
-def get : (e : Env α) → Fin (e.length) → α
+def get : (Γ : Env α) → Fin (Γ.length) → α
   | .cons a _ , ⟨0    , _⟩ => a
   | .cons _ as, ⟨i + 1, h⟩ => as.get ⟨i, Nat.le_of_succ_le_succ h⟩
 
 @[reducible]
-def partition (as : Env α) (mask : List Bool) : Env α × Env α :=
-  go as mask
+def split (Γ : Env α) (mask : List Bool) (h : mask.length = Γ.length) : Env α × Env α :=
+  go Γ mask h
 where
   @[reducible]
-  go : Env α → List Bool → Env α × Env α
-  | .cons a as, b :: bs =>
-    let (ls, rs) := go as bs
-    if b then
-      (.cons a ls, rs)
-    else
-      (ls, .cons a rs)
-  | _, _ =>
-    (.nil, nil)
+  go : (Γ : Env α) → (mask : List Bool) → (mask.length = Γ.length) → Env α × Env α
+  | .nil, .nil, _ => (.nil, nil)
+  | .cons a as, true :: bs, h =>
+    let (ls, rs) := go as bs (length_cons_list_cons h)
+    (.cons a ls, rs)
+  | .cons a as, false :: bs, h =>
+    let (ls, rs) := go as bs (length_cons_list_cons h)
+    (ls, .cons a rs)
 
 @[reducible]
 def toList : Env α → List α
@@ -71,22 +78,25 @@ instance [ToString α] : ToString <| Env α where
 
 end Env
 
+-- Env Theorems
+theorem env_mem_cons_1 [BI PROP] {P : PROP} {Ps : Env PROP} : P ∈ Env.cons P Ps := by
+  simp [Membership.mem, Env.Mem.head]
+
+theorem env_mem_cons_2 [BI PROP] {P Q : PROP} {Ps : Env PROP} : P ∈ Ps → P ∈ Env.cons Q Ps := by
+  intro h_Ps
+  apply Env.Mem.tail
+  exact h_Ps
 
 -- Envs
 structure Envs (PROP : Type) [BI PROP] where
   intuitionistic : Env PROP
   spatial        : Env PROP
 
-def of_envs [BI PROP] (Γₚ Γₛ : Env PROP) : PROP :=
-  match Γₚ, Γₛ with
-  | .nil, .nil => `[iprop| emp]
-  | _   , .nil => `[iprop| □ [∧] Γₚ]
-  | .nil, _    => `[iprop| [∗] Γₛ]
-  | _   , _    => `[iprop| □ [∧] Γₚ ∗ [∗] Γₛ]
+def of_envs [BI PROP] : Envs PROP → PROP
+  | ⟨Γₚ, Γₛ⟩ => `[iprop| □ [∧] Γₚ ∗ [∗] Γₛ]
 
 def envs_entails [BI PROP] (Δ : Envs PROP) (Q : PROP) : Prop :=
-  of_envs Δ.intuitionistic Δ.spatial ⊢ Q
-
+  of_envs Δ ⊢ Q
 
 -- HypothesisIndex
 inductive HypothesisType | intuitionistic | spatial
@@ -100,16 +110,72 @@ inductive EnvsIndex (lₚ lₛ : Nat)
   | p : Fin lₚ → EnvsIndex lₚ lₛ
   | s : Fin lₛ → EnvsIndex lₚ lₛ
 
+abbrev EnvsIndex.of [BI PROP] (Δ : Envs PROP) := EnvsIndex Δ.intuitionistic.length Δ.spatial.length
+
 def HypothesisIndex.quoteAsEnvsIndex : HypothesisIndex → MetaM (TSyntax `term)
   | ⟨.intuitionistic, index, length⟩ =>
     `(EnvsIndex.p ⟨$(quote index), by show $(quote index) < $(quote length) ; decide⟩)
   | ⟨.spatial, index, length⟩ =>
     `(EnvsIndex.s ⟨$(quote index), by show $(quote index) < $(quote length) ; decide⟩)
 
+namespace Envs
+
+@[reducible]
+def concat [BI PROP] : Bool → PROP → Envs PROP → Envs PROP
+  | true,  P, ⟨Γₚ, Γₛ⟩ => ⟨Γₚ.concat P, Γₛ⟩
+  | false, P, ⟨Γₚ, Γₛ⟩ => ⟨Γₚ, Γₛ.concat P⟩
+
+@[reducible]
+def delete [BI PROP] : Bool → (Δ : Envs PROP) → EnvsIndex.of Δ → Envs PROP
+  | true , ⟨Γₚ, Γₛ⟩, .p i => ⟨Γₚ.eraseIdx i, Γₛ⟩
+  | false, ⟨Γₚ, Γₛ⟩, .p _ => ⟨Γₚ, Γₛ⟩
+  | _    , ⟨Γₚ, Γₛ⟩, .s i => ⟨Γₚ, Γₛ.eraseIdx i⟩
+
+@[reducible]
+def lookup [BI PROP] : (Δ : Envs PROP) → EnvsIndex.of Δ → Bool × PROP
+  | ⟨Γₚ, _⟩, .p i => (true, Γₚ.get i)
+  | ⟨_, Γₛ⟩, .s i => (false, Γₛ.get i)
+
+@[reducible]
+def replace [BI PROP] (Δ : Envs PROP) (i : EnvsIndex.of Δ) (p : Bool) (P : PROP) :=
+  Δ.delete true i |>.concat p P
+
+@[reducible]
+def split [BI PROP] : (Δ : Envs PROP) → (mask : List Bool) → (mask.length = Δ.spatial.length) → Envs PROP × Envs PROP
+  | ⟨Γₚ, Γₛ⟩, mask, h =>
+    let ⟨Γₛ₁, Γₛ₂⟩ := Γₛ.split mask h
+    (⟨Γₚ, Γₛ₁⟩, ⟨Γₚ, Γₛ₂⟩)
+
+end Envs
+
+-- Envs Theorems
+theorem envs_concat_sound [BI PROP] {Δ : Envs PROP} (p : Bool) (Q : PROP) :
+  of_envs Δ ⊢ □?p Q -∗ of_envs (Δ.concat p Q)
+:= sorry
+
+theorem envs_lookup_delete_sound [BI PROP] {Δ : Envs PROP} {i : EnvsIndex.of Δ} {p : Bool} {P : PROP} :
+  Δ.lookup i = (p, P) →
+  of_envs Δ ⊢ □?p P ∗ of_envs (Δ.delete true i)
+:= sorry
+
+theorem envs_lookup_replace_sound [BI PROP] {Δ : Envs PROP} {i : EnvsIndex.of Δ} {p : Bool} {P : PROP} (q : Bool) (Q : PROP) :
+  Δ.lookup i = (p, P) →
+  of_envs Δ ⊢ □?p P ∗ (□?q Q -∗ of_envs (Δ.replace i q Q))
+:= sorry
+
+theorem envs_split_sound [BI PROP] {Δ Δ₁ Δ₂ : Envs PROP} {mask : List Bool} {h : mask.length = Δ.spatial.length} :
+  Δ.split mask h = (Δ₁, Δ₂) →
+  of_envs Δ ⊢ of_envs Δ₁ ∗ of_envs Δ₂
+:= sorry
+
+theorem envs_spatial_is_empty_intuitionistically [BI PROP] {Δ : Envs PROP} :
+  Δ.spatial.isEmpty = true → of_envs Δ ⊢ □ of_envs Δ
+:= sorry
 
 -- AffineEnv
 class AffineEnv [BI PROP] (Γ : Env PROP) where
   affineEnv : ∀ P, P ∈ Γ → Affine P
+export AffineEnv (affineEnv)
 
 instance affineEnvNil [BI PROP] :
   AffineEnv (PROP := PROP) .nil
@@ -118,25 +184,40 @@ where
     intro _ h
     cases h
 
-instance affineEnvConcat [BI PROP] (P : PROP) (Γ : Env PROP)
-  [instP : Affine P]
-  [instΓ : AffineEnv Γ] :
+instance affineEnvConcat [BI PROP] (P : PROP) (Γ : Env PROP) :
+  [Affine P] →
+  [AffineEnv Γ] →
   AffineEnv (.cons P Γ)
 where
   affineEnv := by
     intro P h
     cases h
     case head =>
-      exact ⟨instP.affine⟩
+      exact ⟨affine⟩
     case tail h =>
-      exact instΓ.affineEnv P h
+      exact affineEnv P h
 
-instance (priority := default + 10) affineEnvBi (Γ : Env PROP)
-  [inst : BIAffine PROP] :
+instance (priority := default + 10) affineEnvBi (Γ : Env PROP) :
+  [BIAffine PROP] →
   AffineEnv Γ
 where
   affineEnv := by
     intro P _
-    exact inst.affine P
+    exact BIAffine.affine P
+
+scoped instance affineEnvSpatial [BI PROP] (Γ : Env PROP)
+  [inst : AffineEnv Γ] :
+  Affine (`[iprop| [∗] Γ] : PROP)
+where
+  affine := by
+    induction Γ generalizing inst
+    case nil =>
+      rw' [big_sepL_nil]
+    case cons P Ps h_ind =>
+      have : AffineEnv Ps := ⟨by
+        intro P h_Ps
+        exact inst.affineEnv P (env_mem_cons_2 h_Ps)⟩
+      have : Affine P := inst.affineEnv P env_mem_cons_1
+      rw' [big_sepL_cons, h_ind, affine]
 
 end Iris.Proofmode
