src/Iris/Proofmode/Classes.lean
@@ -26,52 +26,68 @@ theorem as_emp_valid_2 (φ : Prop) [AsEmpValid2 φ P] : (⊢ P) → φ :=
 
 class FromImpl [BI PROP] (P : PROP) (Q1 Q2 : outParam PROP) where
   from_impl : (Q1 → Q2) ⊢ P
+export FromImpl (from_impl)
 
 class FromWand [BI PROP] (P : PROP) (Q1 Q2 : outParam PROP) where
   from_wand : (Q1 -∗ Q2) ⊢ P
+export FromWand (from_wand)
 
 class FromForall [BI PROP] (P : PROP) {α : outParam Type} (Ψ : outParam <| α → PROP) where
   from_forall : (∀ x, Ψ x) ⊢ P
+export FromForall (from_forall)
 
 class FromExist [BI PROP] (P : PROP) {α : outParam Type} (Φ : outParam <| α → PROP) where
   from_exist : (∃ x, Φ x) ⊢ P
+export FromExist (from_exist)
 
 class FromAnd [BI PROP] (P : PROP) (Q1 Q2 : outParam PROP) where
   from_and : Q1 ∧ Q2 ⊢ P
+export FromAnd (from_and)
 
 class IntoAnd (p : Bool) [BI PROP] (P : PROP) (Q1 Q2 : outParam PROP) where
   into_and : □?p P ⊢ □?p (Q1 ∧ Q2)
+export IntoAnd (into_and)
 
 class FromSep [BI PROP] (P : PROP) (Q1 Q2 : outParam PROP) where
   from_sep : Q1 ∗ Q2 ⊢ P
+export FromSep (from_sep)
 
 class IntoSep [BI PROP] (P : PROP) (Q1 Q2 : outParam PROP) :=
   into_sep : P ⊢ Q1 ∗ Q2
+export IntoSep (into_sep)
 
 class FromOr [BI PROP] (P : PROP) (Q1 Q2 : outParam PROP) where
   from_or : Q1 ∨ Q2 ⊢ P
+export FromOr (from_or)
 
 class IntoOr [BI PROP] (P : PROP) (Q1 Q2 : outParam PROP) where
   into_or : P ⊢ Q1 ∨ Q2
+export IntoOr (into_or)
 
 
 class IntoPersistent (p : Bool) [BI PROP] (P : PROP) (Q : outParam PROP) where
   into_persistent : <pers>?p P ⊢ <pers> Q
+export IntoPersistent (into_persistent)
 
 class FromAffinely [BI PROP] (P : outParam PROP) (Q : PROP) (p : Bool := true) where
   from_affinely : <affine>?p Q ⊢ P
+export FromAffinely (from_affinely)
 
 class IntoAbsorbingly [BI PROP] (P : outParam PROP) (Q : PROP) where
   into_absorbingly : P ⊢ <absorb> Q
+export IntoAbsorbingly (into_absorbingly)
 
 
 class FromAssumption (p : Bool) [BI PROP] (P Q : PROP) where
   from_assumption : □?p P ⊢ Q
+export FromAssumption (from_assumption)
 
 class IntoPure [BI PROP] (P : PROP) (φ : outParam Prop) where
   into_pure : P ⊢ ⌜φ⌝
+export IntoPure (into_pure)
 
 class FromPure [BI PROP] (a : outParam Bool) (P : PROP) (φ : outParam Prop) where
   from_pure : <affine>?a ⌜φ⌝ ⊢ P
+export FromPure (from_pure)
 
 end Iris.Proofmode
