src/Iris/Proofmode/Theorems.lean
@@ -5,150 +5,391 @@ import Iris.Std.TC
 
 namespace Iris.Proofmode
 open Iris.BI Iris.Std
+open BI
+
+scoped macro "intro_let " names:(colGt Lean.binderIdent)* : tactic => `(
+  intro _ ;
+  split ;
+  rename_i $[$names]*
+)
 
 -- proof mode
 theorem tac_start [BI PROP] (P : PROP) :
   envs_entails ⟨.nil, .nil⟩ P →
   ⊢ P
-:= sorry
+:= by
+  simp only [envs_entails, of_envs, big_op, List.foldr1]
+  rw' [intuitionistically_True_emp, (left_id : emp ∗ _ ⊣⊢ _)]
+  intro h
+  exact h
 
-theorem tac_clear [BI PROP] {Γₚ Γₛ : Env PROP} (i : EnvsIndex Γₚ.length Γₛ.length) (Q : PROP) :
-  let (p, P, Γₚ', Γₛ') := match i with
-    | .p i => (true, Γₚ.get i, Γₚ.eraseIdx i, Γₛ)
-    | .s i => (false, Γₛ.get i, Γₚ, Γₛ.eraseIdx i)
+theorem tac_stop [BI PROP] {Γₚ Γₛ : Env PROP} (P : PROP) :
+  let Ps := match Γₚ, Γₛ with
+    | .nil, .nil => `[iprop| emp]
+    | _   , .nil => `[iprop| □ [∧] Γₚ]
+    | .nil, _    => `[iprop| [∗] Γₛ]
+    | _   , _    => `[iprop| □ [∧] Γₚ ∗ [∗] Γₛ]
+  (Ps ⊢ P) →
+  envs_entails ⟨Γₚ, Γₛ⟩ P
+:= by
+  cases Γₚ
+  <;> cases Γₛ
+  all_goals
+    simp [envs_entails, of_envs, big_op, List.foldr1]
+    intro Ps
+    rw' [Ps]
+  case cons.nil =>
+    rw' [(right_id : _ ∗ emp ⊣⊢ _)]
+  all_goals
+    rw' [intuitionistically_True_emp, (left_id : emp ∗ _ ⊣⊢ _)]
+
+theorem tac_clear [BI PROP] {Δ : Envs PROP} (i : EnvsIndex.of Δ) (Q : PROP) :
+  let (p, P) := Δ.lookup i
   [TCIte p TCTrue (TCOr (Affine P) (Absorbing Q))] →
-  envs_entails ⟨Γₚ', Γₛ'⟩ Q →
-  envs_entails ⟨Γₚ, Γₛ⟩ Q
-:= sorry
+  envs_entails (Δ.delete true i) Q →
+  envs_entails Δ Q
+:= by
+  intro_let p P h_lookup
+  intro inst_affine_absorbing
+  cases p
+  all_goals
+    cases inst_affine_absorbing
+    simp only [envs_entails]
+    intro h_entails
+    rw' [envs_lookup_delete_sound h_lookup, h_entails]
+    simp only [bi_intuitionistically_if, ite_true, ite_false]
+    rw' [sep_elim_r]
 
 -- pure
-theorem tac_pure_intro [BI PROP] {Γₚ Γₛ : Env PROP} {a : Bool} {φ : Prop} (Q : PROP) :
+theorem tac_pure_intro [BI PROP] {Δ : Envs PROP} {a : Bool} {φ : Prop} (Q : PROP) :
   [FromPure a Q φ] →
-  [TCIte a (AffineEnv Γₛ) TCTrue] →
+  [TCIte a (AffineEnv Δ.spatial) TCTrue] →
   φ →
-  envs_entails ⟨Γₚ, Γₛ⟩ Q
-:= sorry
+  envs_entails Δ Q
+:= by
+  simp only [envs_entails]
+  intro _ inst_affine_env hφ
+  rw' [← from_pure]
+  cases a
+  case false =>
+    apply pure_intro
+    exact hφ
+  case true =>
+    cases inst_affine_env
+    simp only [of_envs, bi_affinely_if]
+    rw' [
+      affine,
+      pure_True hφ,
+      affinely_True_emp,
+      affinely_emp]
 
 -- implication and wand
-theorem tac_impl_intro [BI PROP] {Γₚ Γₛ : Env PROP} {P Q : PROP} (R : PROP) :
+theorem tac_impl_intro [BI PROP] {Δ : Envs PROP} {P Q : PROP} (R : PROP) :
   [FromImpl R P Q] →
-  [TCIte Γₛ.isEmpty TCTrue (Persistent P)] →
+  [TCIte Δ.spatial.isEmpty TCTrue (Persistent P)] →
   [FromAffinely P' P] →
-  envs_entails ⟨Γₚ, Γₛ.concat P'⟩ Q →
-  envs_entails ⟨Γₚ, Γₛ⟩ R
-:= sorry
+  envs_entails (Δ.concat false P') Q →
+  envs_entails Δ R
+:= by
+  simp only [envs_entails]
+  intro _ inst_pers _ h_entails
+  rw' [← from_impl]
+  cases h_empty : Δ.spatial.isEmpty
+  <;> rw [h_empty] at inst_pers
+  <;> cases inst_pers
+  case false =>
+    apply impl_intro_l
+    rw' [
+      envs_concat_sound false P',
+      (from_affinely : <affine>?true P ⊢ _),
+      persistent_and_affinely_sep_l_1,
+      wand_elim_r,
+      h_entails]
+  case true =>
+    rw' [envs_spatial_is_empty_intuitionistically h_empty]
+    apply impl_intro_l
+    rw' [
+      envs_concat_sound false P',
+      (from_affinely : <affine>?true P ⊢ _)]
+    simp only [bi_intuitionistically]
+    rw' [
+      ← affinely_and_lr,
+      persistently_and_intuitionistically_sep_r,
+      intuitionistically_elim,
+      wand_elim_r,
+      h_entails]
 
-theorem tac_impl_intro_intuitionistic [BI PROP] {Γₚ Γₛ : Env PROP} {P P' Q : PROP} (R : PROP) :
+theorem tac_impl_intro_intuitionistic [BI PROP] {Δ : Envs PROP} {P P' Q : PROP} (R : PROP) :
   [FromImpl R P Q] →
   [IntoPersistent false P P'] →
-  envs_entails ⟨Γₚ.concat P', Γₛ⟩ Q →
-  envs_entails ⟨Γₚ, Γₛ⟩ R
-:= sorry
+  envs_entails (Δ.concat true P') Q →
+  envs_entails Δ R
+:= by
+  simp only [envs_entails]
+  intro _ _ h_entails
+  rw' [← from_impl, envs_concat_sound true P'] ; simp only
+  apply impl_intro_l
+  rw' [
+    persistently_if_intro_False P,
+    into_persistent,
+    persistently_and_intuitionistically_sep_l,
+    wand_elim_r,
+    h_entails]
 
 theorem tac_impl_intro_drop [BI PROP] {Δ : Envs PROP} {P Q : PROP} (R : PROP) :
   [FromImpl R P Q] →
   envs_entails Δ Q →
   envs_entails Δ R
-:= sorry
+:= by
+  simp only [envs_entails]
+  intro _ h_entails
+  rw' [← from_impl]
+  apply impl_intro_l
+  rw' [and_elim_r, h_entails]
 
-theorem tac_wand_intro [BI PROP] {Γₚ Γₛ : Env PROP} {P Q : PROP} (R : PROP) :
+theorem tac_wand_intro [BI PROP] {Δ : Envs PROP} {P Q : PROP} (R : PROP) :
   [FromWand R P Q] →
-  envs_entails ⟨Γₚ, Γₛ.concat P⟩ Q →
-  envs_entails ⟨Γₚ, Γₛ⟩ R
-:= sorry
+  envs_entails (Δ.concat false P) Q →
+  envs_entails Δ R
+:= by
+  simp only [envs_entails]
+  intro _ h_entails
+  rw' [
+    ← from_wand,
+    envs_concat_sound false P,
+    h_entails]
 
-theorem tac_wand_intro_intuitionistic [BI PROP] {Γₚ Γₛ : Env PROP} {P P' Q : PROP} (R : PROP) :
+theorem tac_wand_intro_intuitionistic [BI PROP] {Δ : Envs PROP} {P P' Q : PROP} (R : PROP) :
   [FromWand R P Q] →
   [IntoPersistent false P P'] →
   [TCOr (Affine P) (Absorbing Q)] →
-  envs_entails ⟨Γₚ.concat P', Γₛ⟩ Q →
-  envs_entails ⟨Γₚ, Γₛ⟩ R
-:= sorry
+  envs_entails (Δ.concat true P') Q →
+  envs_entails Δ R
+:= by
+  simp only [envs_entails]
+  intro _ _ inst_affine_absorbing h_entails
+  rw' [← from_wand, envs_concat_sound true P'] ; simp only
+  apply wand_intro_l
+  cases inst_affine_absorbing
+  case a.l =>
+    rw' [
+      ← (affine_affinely : _ ⊣⊢ P),
+      persistently_if_intro_False P,
+      into_persistent,
+      wand_elim_r,
+      h_entails]
+  case a.r =>
+    rw' [
+      persistently_if_intro_False P,
+      into_persistent,
+      ← absorbingly_intuitionistically_into_persistently,
+      absorbingly_sep_l,
+      wand_elim_r,
+      h_entails,
+      absorbing]
 
 -- forall
 theorem tac_forall_intro [BI PROP] {Δ : Envs PROP} {Ψ : α → PROP} (Q : PROP) :
   [FromForall Q Ψ] →
   (∀ a, envs_entails Δ `[iprop| Ψ a]) →
   envs_entails Δ Q
-:= sorry
+:= by
+  simp only [envs_entails]
+  intro _ h_entails
+  rw' [← from_forall]
+  apply forall_intro
+  exact h_entails
 
 -- exist
 theorem tac_exist [BI PROP] {Δ : Envs PROP} {Φ : α → PROP} (P : PROP) :
   [FromExist P Φ] →
   (∃ a, envs_entails Δ `[iprop| Φ a]) →
   envs_entails Δ P
-:= sorry
+:= by
+  simp only [envs_entails]
+  intro _ ⟨a, h_entails⟩
+  rw' [← from_exist, ← exist_intro a, h_entails]
 
 -- assumptions
-theorem tac_assumption_lean [BI PROP] {Γₚ Γₛ : Env PROP} {P : PROP} (Q : PROP) :
+theorem tac_assumption_lean [BI PROP] {Δ : Envs PROP} {P : PROP} (Q : PROP) :
   (⊢ P) →
   [FromAssumption true P Q] →
-  [TCIte Γₛ.isEmpty TCTrue (TCOr (Absorbing Q) (AffineEnv Γₛ))] →
-  envs_entails ⟨Γₚ, Γₛ⟩ Q
-:= sorry
+  [TCIte Δ.spatial.isEmpty TCTrue (TCOr (Absorbing Q) (AffineEnv Δ.spatial))] →
+  envs_entails Δ Q
+:= by
+  simp only [envs_entails]
+  intro h_P _ inst_absorbing_affine_env
+  rw' [
+    ← (left_id : emp ∗ of_envs Δ ⊣⊢ _),
+    ← intuitionistically_emp,
+    h_P,
+    (from_assumption : □?true P ⊢ Q)]
+  cases h_empty : Δ.spatial.isEmpty
+  <;> rw [h_empty] at inst_absorbing_affine_env
+  <;> cases inst_absorbing_affine_env
+  case false.e inst_absorbing_affine_env =>
+    cases inst_absorbing_affine_env
+    <;> rw' [!sep_elim_l]
+  case true.t =>
+    rw' [envs_spatial_is_empty_intuitionistically h_empty, sep_elim_l]
 
-theorem tac_assumption [BI PROP] {Γₚ Γₛ : Env PROP} (i : EnvsIndex Γₚ.length Γₛ.length) (Q : PROP) :
-  let (p, P) := match i with
-    | .p i => (true, Γₚ.get i)
-    | .s i => (false, Γₛ.get i)
+theorem tac_assumption [BI PROP] {Δ : Envs PROP} (i : EnvsIndex.of Δ) (Q : PROP) :
+  let (p, P) := Δ.lookup i
   [FromAssumption p P Q] →
-  let Γₛ' := if let .s i := i then Γₛ.eraseIdx i else Γₛ
-  [TCIte Γₛ'.isEmpty TCTrue (TCOr (Absorbing Q) (AffineEnv Γₛ'))] →
-  envs_entails ⟨Γₚ, Γₛ⟩ Q
-:= sorry
+  let Δ' := Δ.delete true i
+  [TCIte Δ'.spatial.isEmpty TCTrue (TCOr (Absorbing Q) (AffineEnv Δ'.spatial))] →
+  envs_entails Δ Q
+:= by
+  intro_let p P h_lookup
+  simp only [envs_entails]
+  intro _ inst_absorbing_affine_env
+  rw' [envs_lookup_delete_sound h_lookup]
+  cases h_empty : (Δ.delete true i).spatial.isEmpty
+  <;> rw [h_empty] at inst_absorbing_affine_env
+  <;> cases inst_absorbing_affine_env
+  case false.e inst_absorbing_affine_env =>
+    rw' [(from_assumption : □?p P ⊢ Q)]
+    cases inst_absorbing_affine_env
+    <;> rw' [!sep_elim_l]
+  case true.t =>
+    rw' [envs_spatial_is_empty_intuitionistically h_empty, sep_elim_l]
+    exact from_assumption
 
 -- false
 theorem tac_ex_falso [BI PROP] {Δ : Envs PROP} (Q : PROP) :
   envs_entails Δ `[iprop| False] →
   envs_entails Δ Q
-:= sorry
+:= by
+  simp only [envs_entails]
+  intro h_entails
+  rw' [h_entails]
+  exact False_elim
 
-theorem tac_false_destruct [BI PROP] {Γₚ Γₛ : Env PROP} (i : EnvsIndex Γₚ.length Γₛ.length) (Q : PROP) :
-  let P := match i with
-    | .p i => Γₚ.get i
-    | .s i => Γₛ.get i
+theorem tac_false_destruct [BI PROP] {Δ : Envs PROP} (i : EnvsIndex.of Δ) (Q : PROP) :
+  let (_, P) := Δ.lookup i
   P = `[iprop| False] →
-  envs_entails ⟨Γₚ, Γₛ⟩ Q
-:= sorry
+  envs_entails Δ Q
+:= by
+  intro_let p P h_lookup
+  simp only [envs_entails]
+  intro h_false
+  rw' [
+    envs_lookup_delete_sound h_lookup,
+    intuitionistically_if_elim,
+    h_false,
+    sep_elim_l]
+  exact False_elim
 
 -- moving between contexts
-theorem tac_pure [BI PROP] {Γₚ Γₛ : Env PROP} {φ : Prop} (i : EnvsIndex Γₚ.length Γₛ.length) (Q : PROP) :
-   let (p, P) := match i with
-    | .p i => (true, Γₚ.get i)
-    | .s i => (false, Γₛ.get i)
+theorem tac_pure [BI PROP] {Δ : Envs PROP} {φ : Prop} (i : EnvsIndex.of Δ) (Q : PROP) :
+   let (p, P) := Δ.lookup i
   [IntoPure P φ] →
   [TCIte p TCTrue (TCOr (Affine P) (Absorbing Q))] →
-   let (Γₚ', Γₛ') := match i with
-    | .p i => (Γₚ.eraseIdx i, Γₛ)
-    | .s i => (Γₚ, Γₛ.eraseIdx i)
-  (φ → envs_entails ⟨Γₚ', Γₛ'⟩ Q) →
-  envs_entails ⟨Γₚ, Γₛ⟩ Q
-:= sorry
+  (φ → envs_entails (Δ.delete true i) Q) →
+  envs_entails Δ Q
+:= by
+  intro_let p P h_lookup
+  simp only [envs_entails]
+  intro _ inst_affine_absorbing h_entails
+  rw' [envs_lookup_delete_sound h_lookup]
+  cases p
+  <;> simp only [bi_intuitionistically_if, ite_true, ite_false]
+  <;> cases inst_affine_absorbing
+  case false.e inst_affine_absorbing =>
+    cases inst_affine_absorbing
+    case l =>
+      rw' [
+        ← (affine_affinely : _ ⊣⊢ P),
+        into_pure,
+        ← persistent_and_affinely_sep_l]
+      apply pure_elim φ
+      · exact and_elim_l
+      · intro h_φ
+        rw' [h_entails h_φ, and_elim_r]
+    case r =>
+      rw' [
+        into_pure,
+        persistent_absorbingly_affinely_2,
+        absorbingly_sep_lr,
+        ← persistent_and_affinely_sep_l]
+      apply pure_elim_l
+      intro h_φ
+      rw' [h_entails h_φ, absorbing]
+  case true.t =>
+    rw' [
+      into_pure,
+      ← persistently_and_intuitionistically_sep_l,
+      persistently_pure]
+    apply pure_elim_l
+    intro h_φ
+    rw' [h_entails h_φ]
 
-theorem tac_intuitionistic [BI PROP] {Γₚ Γₛ : Env PROP} {P' : PROP} (i : EnvsIndex Γₚ.length Γₛ.length) (Q : PROP) :
-  let (p, P) := match i with
-    | .p i => (true, Γₚ.get i)
-    | .s i => (false, Γₛ.get i)
+theorem tac_intuitionistic [BI PROP] {Δ : Envs PROP} {P' : PROP} (i : EnvsIndex.of Δ) (Q : PROP) :
+  let (p, P) := Δ.lookup i
   [IntoPersistent p P P'] →
   [TCIte p TCTrue (TCOr (Affine P) (Absorbing Q))] →
-  let (Γₚ', Γₛ') := match i with
-    | .p i => (Γₚ |>.eraseIdx i |>.concat P', Γₛ)
-    | .s i => (Γₚ.concat P', Γₛ.eraseIdx i)
-  envs_entails ⟨Γₚ', Γₛ'⟩ Q →
-  envs_entails ⟨Γₚ, Γₛ⟩ Q
-:= sorry
+  envs_entails (Δ.replace i true P') Q →
+  envs_entails Δ Q
+:= by
+  intro_let p P h_lookup
+  simp only [envs_entails]
+  intro _ inst_affine_absorbing h_entails
+  rw' [envs_lookup_replace_sound true P' h_lookup]
+  cases p
+  <;> simp only [bi_intuitionistically_if, ite_true, ite_false, bi_intuitionistically]
+  <;> cases inst_affine_absorbing
+  case false inst_affine_absorbing =>
+    cases inst_affine_absorbing
+    case l =>
+      rw' [
+        ← (affine_affinely : _ ⊣⊢ P),
+        persistently_if_intro_False P,
+        into_persistent,
+        wand_elim_r,
+        h_entails]
+    case r =>
+      rw' [persistently_if_intro_False P, into_persistent]
+      conv =>
+        lhs
+        lhs
+        rw [← absorbingly_intuitionistically_into_persistently]
+      rw' [
+        absorbingly_sep_l,
+        wand_elim_r,
+        h_entails,
+        absorbing]
+  case true =>
+    rw' [
+      persistently_if_intro_True P,
+      into_persistent,
+      wand_elim_r,
+      h_entails]
 
-theorem tac_spatial [BI PROP] {Γₚ Γₛ : Env PROP} {P' : PROP} (i : EnvsIndex Γₚ.length Γₛ.length) (Q : PROP) :
-  let (p, P) := match i with
-    | .p i => (true, Γₚ.get i)
-    | .s i => (false, Γₛ.get i)
+theorem tac_spatial [BI PROP] {Δ : Envs PROP} {P' : PROP} (i : EnvsIndex.of Δ) (Q : PROP) :
+  let (p, P) := Δ.lookup i
   [FromAffinely P' P p] →
-  let (Γₚ', Γₛ') := match i with
-    | .p i => (Γₚ.eraseIdx i, Γₛ.concat P')
-    | .s i => (Γₚ, Γₛ |>.eraseIdx i |>.concat P')
-  envs_entails ⟨Γₚ', Γₛ'⟩ Q →
-  envs_entails ⟨Γₚ, Γₛ⟩ Q
-:= sorry
+  envs_entails (Δ.replace i false P') Q →
+  envs_entails Δ Q
+:= by
+  intro_let p P h_lookup
+  simp only [envs_entails]
+  intro _ h_entails
+  rw' [envs_lookup_replace_sound false P' h_lookup]
+  cases p
+  <;> simp only [bi_intuitionistically_if, ite_true, ite_false]
+  case false =>
+    rw' [
+      affinely_if_intro_False P,
+      from_affinely,
+      wand_elim_r,
+      h_entails]
+  case true =>
+    rw' [
+      intuitionistically_affinely,
+      affinely_if_intro_True P,
+      from_affinely,
+      wand_elim_r,
+      h_entails]
 
 -- (separating) conjunction splitting
 theorem tac_and_split [BI PROP] {Δ : Envs PROP} {Q1 Q2 : PROP} (P : PROP) :
@@ -156,28 +397,52 @@ theorem tac_and_split [BI PROP] {Δ : Envs PROP} {Q1 Q2 : PROP} (P : PROP) :
   envs_entails Δ Q1 →
   envs_entails Δ Q2 →
   envs_entails Δ P
-:= sorry
+:= by
+  simp only [envs_entails]
+  intro _ h_entails_1 h_entails_2
+  rw' [← from_and]
+  apply and_intro
+  · exact h_entails_1
+  · exact h_entails_2
 
-theorem tac_sep_split [BI PROP] {Γₚ Γₛ : Env PROP} {Q1 Q2 : PROP} (mask : List Bool) (P : PROP) :
+theorem tac_sep_split [BI PROP] {Δ : Envs PROP} {Q1 Q2 : PROP} (mask : List Bool) (h : mask.length = Δ.spatial.length) (P : PROP) :
+  let (Δ₁, Δ₂) := Δ.split mask h
   [FromSep P Q1 Q2] →
-  let (Γₛ₁, Γₛ₂) := Γₛ.partition mask
-  envs_entails ⟨Γₚ, Γₛ₁⟩ Q1 →
-  envs_entails ⟨Γₚ, Γₛ₂⟩ Q2 →
-  envs_entails ⟨Γₚ, Γₛ⟩ P
-:= sorry
+  envs_entails Δ₁ Q1 →
+  envs_entails Δ₂ Q2 →
+  envs_entails Δ P
+:= by
+  intro_let Δ₁ Δ₂ h_split
+  simp only [envs_entails]
+  intro _ h_entails_1 h_entails_2
+  rw' [
+    envs_split_sound h_split,
+    ← from_sep,
+    h_entails_1,
+    h_entails_2]
 
 -- disjunction selection
 theorem tac_disjunction_l [BI PROP] {Δ : Envs PROP} {Q1 Q2 : PROP} (P : PROP) :
   [FromOr P Q1 Q2] →
   envs_entails Δ Q1 →
   envs_entails Δ P
-:= sorry
+:= by
+  simp only [envs_entails]
+  intro _ h_entails
+  rw' [← from_or]
+  apply or_intro_l'
+  exact h_entails
 
 theorem tac_disjunction_r [BI PROP] {Δ : Envs PROP} {Q1 Q2 : PROP} (P : PROP) :
   [FromOr P Q1 Q2] →
   envs_entails Δ Q2 →
   envs_entails Δ P
-:= sorry
+:= by
+  simp only [envs_entails]
+  intro _ h_entails
+  rw' [← from_or]
+  apply or_intro_r'
+  exact h_entails
 
 -- destruction
 class inductive IntoConjunction [BI PROP] (P : PROP) (P1 P2 : outParam PROP) : Bool → Type
@@ -187,46 +452,83 @@ class inductive IntoConjunction [BI PROP] (P : PROP) (P1 P2 : outParam PROP) : B
 attribute [instance] IntoConjunction.and
 attribute [instance] IntoConjunction.sep
 
-theorem tac_conjunction_destruct [BI PROP] {Γₚ Γₛ : Env PROP} {P1 P2 : PROP} (i : EnvsIndex Γₚ.length Γₛ.length) (Q : PROP) :
-  let (p, P) := match i with
-    | .p i => (true, Γₚ.get i)
-    | .s i => (false, Γₛ.get i)
+theorem tac_conjunction_destruct [BI PROP] {Δ : Envs PROP} {P1 P2 : PROP} (i : EnvsIndex.of Δ) (Q : PROP) :
+  let (p, P) := Δ.lookup i
   [IntoConjunction P P1 P2 p] →
-  let (Γₚ', Γₛ') := match i with
-    | .p i => (Γₚ |>.eraseIdx i |>.concat P1 |>.concat P2, Γₛ)
-    | .s i => (Γₚ, Γₛ |>.eraseIdx i |>.concat P1 |>.concat P2)
-  envs_entails ⟨Γₚ', Γₛ'⟩ Q →
-  envs_entails ⟨Γₚ, Γₛ⟩ Q
-:= sorry
+  envs_entails (Δ |>.delete true i |>.concat p P1 |>.concat p P2) Q →
+  envs_entails Δ Q
+:= by
+  intro_let p P h_lookup
+  simp only [envs_entails]
+  intro inst_conjunction h_entails
+  rw' [
+    envs_lookup_delete_sound h_lookup,
+    envs_concat_sound p P1,
+    envs_concat_sound p P2] ; simp only
+  cases p
+  <;> simp only [bi_intuitionistically_if, ite_true, ite_false]
+  <;> cases inst_conjunction
+  case false.sep =>
+    rw' [
+      into_sep,
+      (comm : P1 ∗ P2 ⊣⊢ _),
+      ← (assoc : _ ⊣⊢ (P2 ∗ P1) ∗ _),
+      wand_elim_r,
+      wand_elim_r,
+      h_entails]
+  case true.and =>
+    rw' [intuitionistically_if_intro_True P, into_and]
+    simp only [bi_intuitionistically_if, ite_true]
+    rw' [
+      intuitionistically_and,
+      and_sep_intuitionistically,
+      (comm : □ P1 ∗ □ P2 ⊣⊢ _),
+      ← (assoc : _ ⊣⊢ (□ P2 ∗ □ P1) ∗ _),
+      wand_elim_r,
+      wand_elim_r,
+      h_entails]
 
-theorem tac_conjunction_destruct_choice [BI PROP] {Γₚ Γₛ : Env PROP} {P1 P2 : PROP} (i : EnvsIndex Γₚ.length Γₛ.length) (d : Bool) (Q : PROP) :
-  let (p, P) := match i with
-    | .p i => (true, Γₚ.get i)
-    | .s i => (false, Γₛ.get i)
+theorem tac_conjunction_destruct_choice [BI PROP] {Δ : Envs PROP} {P1 P2 : PROP} (i : EnvsIndex.of Δ) (d : Bool) (Q : PROP) :
+  let (p, P) := Δ.lookup i
   [IntoAnd p P P1 P2] →
-  let P' := if d then P1 else P2
-  let (Γₚ', Γₛ') := match i with
-    | .p i => (Γₚ |>.eraseIdx i |>.concat P', Γₛ)
-    | .s i => (Γₚ, Γₛ |>.eraseIdx i |>.concat P')
-  envs_entails ⟨Γₚ', Γₛ'⟩ Q →
-  envs_entails ⟨Γₚ, Γₛ⟩ Q
-:= sorry
+  envs_entails (if d then Δ.replace i p P1 else Δ.replace i p P2) Q →
+  envs_entails Δ Q
+:= by
+  intro_let p P h_lookup
+  simp only [envs_entails]
+  intro _ h_entails
+  cases d
+  case false =>
+    rw' [
+      envs_lookup_replace_sound p P2 h_lookup,
+      into_and,
+      and_elim_r,
+      wand_elim_r,
+      h_entails]
+  case true =>
+    rw' [
+      envs_lookup_replace_sound p P1 h_lookup,
+      into_and,
+      and_elim_l,
+      wand_elim_r,
+      h_entails]
 
-theorem tac_disjunction_destruct [BI PROP] {Γₚ Γₛ : Env PROP} {P1 P2 : PROP} (i : EnvsIndex Γₚ.length Γₛ.length) (Q : PROP) :
-  let P := match i with
-    | .p i => Γₚ.get i
-    | .s i => Γₛ.get i
+theorem tac_disjunction_destruct [BI PROP] {Δ : Envs PROP} {P1 P2 : PROP} (i : EnvsIndex.of Δ) (Q : PROP) :
+  let (p, P) := Δ.lookup i
   [IntoOr P P1 P2] →
-  let (Γₚₗ, Γₚᵣ, Γₛₗ, Γₛᵣ) := match i with
-    | .p i => (
-      Γₚ |>.eraseIdx i |>.concat P1, Γₚ |>.eraseIdx i |>.concat P2,
-      Γₛ, Γₛ)
-    | .s i => (
-      Γₚ, Γₚ,
-      Γₛ |>.eraseIdx i |>.concat P1, Γₛ |>.eraseIdx i |>.concat P2)
-  envs_entails ⟨Γₚₗ, Γₛₗ⟩ Q →
-  envs_entails ⟨Γₚᵣ, Γₛᵣ⟩ Q →
-  envs_entails ⟨Γₚ, Γₛ⟩ Q
-:= sorry
+  envs_entails (Δ.replace i p P1) Q →
+  envs_entails (Δ.replace i p P2) Q →
+  envs_entails Δ Q
+:= by
+  intro_let p P h_lookup
+  simp only [envs_entails]
+  intro _ h_entails_1 h_entails_2
+  rw' [envs_lookup_delete_sound h_lookup] ; simp only
+  simp only [Envs.replace] at h_entails_1
+  simp only [Envs.replace] at h_entails_2
+  rw' [into_or, intuitionistically_if_or, sep_or_r]
+  apply or_elim
+  · rw' [envs_concat_sound p P1, wand_elim_r, h_entails_1]
+  · rw' [envs_concat_sound p P2, wand_elim_r, h_entails_2]
 
 end Iris.Proofmode
